vaddb + vevictb

steel/Veritas.Steel.Verifier.fsti
@@ -36,7 +36,13 @@ let v_hash (#p:vprop) (r:prf_set_hash)
   : GTot model_hash
   = h (prf_set_hash_inv r)
 
-let thread_id = U32.t
+val prf_update_hash (p:prf_set_hash) (r:T.record) (t:T.timestamp) (thread_id:thread_id)
+  : Steel unit
+    (prf_set_hash_inv p)
+    (fun _ -> prf_set_hash_inv p)
+    (requires fun _ -> True)
+    (ensures fun h0 _ h1 -> v_hash p h1 == model_update_hash (v_hash p h0) r t thread_id)
+
 let counter_t = ref U64.t
 
 noeq
@@ -69,6 +75,15 @@ let v_thread (#p:vprop) (t:thread_state_t)
       model_hadd = v_hash t.hadd (focus_rmem h (thread_state_inv t));
       model_hevict = v_hash t.hevict (focus_rmem h (thread_state_inv t))
     }
+
+// AF: Requires some integers reasoningm, but should be straightforward
+val update_clock (ts:T.timestamp) (vs:thread_state_t)
+  : Steel unit
+    (thread_state_inv vs)
+    (fun _ -> thread_state_inv vs)
+    (requires fun _ -> True)
+    (ensures fun h0 _ h1 -> v_thread vs h1 == model_update_clock (v_thread vs h0) ts)
+
 
 let fail (vs:thread_state_t) (msg:string)
   : SteelF unit
@@ -116,3 +131,70 @@ let vput (s:U32.t) (v:T.value) (vs: thread_state_t)
     | Some r ->
       vcache_update_record vs.st s ({ r with T.record_value = v });
       ()
+
+let vaddb (s:U32.t)
+          (r:T.record)
+          (t:T.timestamp)
+          (thread_id:thread_id)
+          (vs:thread_state_t)
+  : Steel unit
+    (thread_state_inv vs)
+    (fun _ -> thread_state_inv vs)
+    (requires fun h -> U32.v s < length (v_thread vs h).model_store)
+    (ensures fun h0 _ h1 ->
+      U32.v s < length (v_thread vs h0).model_store /\
+      v_thread vs h1 == vaddb_model (v_thread vs h0) s r t thread_id)
+  = let h = get() in
+    assert (U32.v s < length (v_thread vs h).model_store);
+    (* epoch of timestamp of last evict *)
+    let e = epoch_of_timestamp t in
+    let { T.record_key = k;
+          T.record_value = v } = r in
+    (* check value type consistent with key k *)
+    if not (is_value_of k v)
+    then (
+      fail vs "vaddm: value is incompatible with key"
+    )
+    else (
+      let ro = VCache.vcache_get_record vs.st s in
+      if Some? ro
+      then (
+        fail vs "vaddm: slot s already exists"
+      )
+      else (
+        prf_update_hash vs.hadd r t thread_id;// vs;
+        update_clock t vs;
+        VCache.vcache_add_record vs.st s k v T.BAdd)
+    )
+
+let vevictb (s:U32.t)
+            (t:T.timestamp)
+            (vs:thread_state_t)
+  : Steel unit
+    (thread_state_inv vs)
+    (fun _ -> thread_state_inv vs)
+    (requires fun h -> U32.v s < length (v_thread vs h).model_store)
+    (ensures  fun h0 _ h1 ->
+      U32.v s < length (v_thread vs h0).model_store /\
+      v_thread vs h1 == vevictb_model (v_thread vs h0) s t vs.id)
+  = let h = get() in
+    assert (U32.v s < length (v_thread vs h).model_store);
+    let clk = read vs.clock in
+    if not (clk `timestamp_lt` t)
+    then (
+      fail vs "Timestamp is old"
+    )
+    else (
+      (* check that the vstore contains s *)
+      let r = VCache.vcache_get_record vs.st s in
+      match r with
+      | None ->
+        fail vs "Slot is empty"
+
+      | Some r ->
+        (* update the evict hash *)
+        prf_update_hash vs.hevict r t vs.id;
+
+        update_clock t vs;
+
+        VCache.vcache_evict_record vs.st s)
