steel/Veritas.Steel.VerifierModel.fst
@@ -1,6 +1,7 @@
 module Veritas.Steel.VerifierModel
 
 open FStar.Ghost
+module U16 = FStar.UInt16
 module U32 = FStar.UInt32
 module U64 = FStar.UInt64
 
@@ -9,6 +10,7 @@ module T = Veritas.Formats.Types
 
 let data_key = T.key
 let data_value = T.data_value
+let thread_id = U16.t
 
 let contents = Seq.seq (option T.record)
 let model_hash = erased MSH.mset_ms_hashfn_dom
@@ -49,3 +51,74 @@ let vput_model (tsm:thread_state_model) (s:slot tsm) (v:T.value) : thread_state_
   = match model_get_record tsm s with
     | None -> model_fail tsm
     | Some r -> model_put_record tsm s ({r with T.record_value = v})
+
+assume
+val epoch_of_timestamp (t:T.timestamp) : U32.t
+assume
+val is_value_of (k:T.key) (v:T.value) : bool
+assume
+val is_data_key (k:T.key) : bool
+
+let mk_record (k:T.key) (v:T.value{is_value_of k v}) (a:T.add_method) : T.record
+  = {
+      T.record_key = k;
+      T.record_value = v;
+      T.record_add_method = a;
+      T.record_l_child_in_store = T.Vfalse;
+      T.record_r_child_in_store = T.Vfalse
+    }
+
+let model_update_clock (tsm:thread_state_model) (ts:T.timestamp)
+  : thread_state_model
+  = if FStar.UInt.fits (U64.v tsm.model_clock + U64.v ts) 64
+    then { tsm with model_clock = tsm.model_clock `U64.add` ts } //+1
+    else model_fail tsm
+
+assume
+val model_update_hash (h:model_hash) (r:T.record) (t:T.timestamp) (thread_id:thread_id)
+  : model_hash
+
+let model_update_hadd (tsm:_) (r:T.record) (t:T.timestamp) (thread_id:thread_id) =
+  ({tsm with model_hadd = model_update_hash tsm.model_hadd r t thread_id})
+
+let model_update_hevict (tsm:_) (r:T.record) (t:T.timestamp) (thread_id:thread_id) =
+  ({tsm with model_hevict = model_update_hash tsm.model_hevict r t thread_id})
+
+let vaddb_model (tsm:thread_state_model) (s:slot tsm) (r:T.record) (t:T.timestamp) (thread_id:thread_id)
+  : thread_state_model
+  = let e = epoch_of_timestamp t in
+    let { T.record_key = k;
+          T.record_value = v } = r in
+    (* check value type consistent with key k *)
+    if not (is_value_of k v) then model_fail tsm
+    else if Some? (model_get_record tsm s) then model_fail tsm
+    else (
+      //TODO: need to check that the key does not exist
+      (* updated h_add *)
+      let tsm = model_update_hadd tsm r t thread_id in
+      (* updated clock *)
+      let tsm = model_update_clock tsm t in
+      (* add record to store *)
+      model_put_record tsm s (mk_record k v T.BAdd)
+    )
+
+let timestamp_lt (t0 t1:T.timestamp) = t0 `U64.lt` t1
+
+let vevictb_model (tsm:thread_state_model) (s:slot tsm) (t:T.timestamp) (thread_id:thread_id)
+  : GTot thread_state_model
+  = let e = epoch_of_timestamp t in
+    let clk = tsm.model_clock in
+    if not (clk `timestamp_lt` t)
+    then model_fail tsm
+    else begin
+      (* check that the vstore contains s *)
+      match model_get_record tsm s with
+      | None -> model_fail tsm
+      | Some r ->
+        (* update the evict hash *)
+        let tsm = model_update_hevict tsm r t thread_id in
+        (* advance clock to t *)
+        let tsm = model_update_clock tsm t in
+        (* evict record *)
+        model_evict_record tsm s
+    end
